formal/hol4/F4FPPVerifyEndToEndProgramSuccessStackGoalsScript.sml
@@ -60,6 +60,34 @@ Proof
   \\ metis_tac[obligations_stack_imply_equivalence]
 QED
 
+Theorem program_success_implies_equivalence_via_obligation_stack_paramhash_atlas_eq:
+  !g dirac.
+    atlas_eq_is_hol_eq /\ atlas_hash_eq_ok /\ ~group_is_compact g /\
+    fast_program_succeeds g dirac /\ slow_program_succeeds g ==>
+      U_slow g (D_slow g) = U_fast g /\
+      bottom_layer_total_ok g dirac (U_fast g)
+Proof
+  rpt gen_tac
+  \\ rpt strip_tac
+
+  \\ drule fast_program_succeeds_imp_phase_success
+  \\ disch_then strip_assume_tac
+
+  \\ `fast_compute_domain_ok g` by
+       metis_tac[fast_compute_program_succeeds_imp_fast_compute_domain_ok]
+
+  \\ `paramhash_obligations_state_factored_atlas_eq g` by
+       metis_tac[fast_compute_program_succeeds_imp_paramhash_obligations_state_factored_atlas_eq]
+
+  \\ `bottom_layer_ok_param_set g dirac (fast_param_set g)` by
+       metis_tac[bottom_layer_program_succeeds_imp_bottom_layer_ok_param_set_decomposed]
+
+  \\ `slow_refinement_ok g /\ slow_ok_components g` by
+       metis_tac[slow_program_succeeds_imp_refined_slow_obligations_detailed]
+
+  \\ metis_tac[obligations_stack_imply_equivalence_paramhash_atlas_eq]
+QED
+
 (* A convenient specialization for the concrete target group `F4s`. *)
 Theorem program_success_implies_equivalence_via_obligation_stack_F4s:
   !dirac.
@@ -72,6 +100,21 @@ Proof
   \\ rpt strip_tac
   \\ metis_tac
       [ program_success_implies_equivalence_via_obligation_stack
+      , F4s_not_compact
+      ]
+QED
+
+Theorem program_success_implies_equivalence_via_obligation_stack_paramhash_atlas_eq_F4s:
+  !dirac.
+    atlas_eq_is_hol_eq /\ atlas_hash_eq_ok /\
+    fast_program_succeeds F4s dirac /\ slow_program_succeeds F4s ==>
+      U_slow F4s (D_slow F4s) = U_fast F4s /\
+      bottom_layer_total_ok F4s dirac (U_fast F4s)
+Proof
+  rpt gen_tac
+  \\ rpt strip_tac
+  \\ metis_tac
+      [ program_success_implies_equivalence_via_obligation_stack_paramhash_atlas_eq
       , F4s_not_compact
       ]
 QED
